\documentclass[a4paper]{article}

\def\npart{IB}

\def\ntitle{Groups, Rings and Modules}
\def\nlecturer{O.\ Randal-Williams}

\def\nterm{Lent}
\def\nyear{2017}

\input{header}

\DeclareMathOperator{\Ann}{Ann}

\makeindex

\begin{document}

\input{titlepage}

\tableofcontents

\section{Groups}

\subsection{Definitions}

\begin{definition}[Group]\index{group}
  A \emph{group} is a triple \((G, \cdot, e)\) of a set \(G\), a function \(- \cdot -: G \times G \to G\) and \(e \in G\) such that
  \begin{itemize}
  \item associativity: for all \(a, b, c \in G\), \((a \cdot b) \cdot c = a \cdot (b \cdot c)\),
  \item identity: for all \(a \in G\), \(a \cdot e = a = e \cdot a\),
  \item inverse: for all \(a \in G\), there exists \(\alpha^{-1} \in G\) such that \(a \cdot a^{-1} = e = a^{-1} \cdot a\).
  \end{itemize}
\end{definition}

\begin{definition}[Subgroup]\index{group!subgroup}
  If \((G, \cdot, e)\) is a group, \(H \subseteq G\) is a \emph{subgroup} if
  \begin{itemize}
  \item \(e \in H\),
  \item for all \(a, b \in H\), \(a \cdot b \in H\).
  \end{itemize}
  This makes \((H, \cdot, e)\) into a group. Write \(H \leq G\).
\end{definition}

\begin{lemma}
  If \(H \subseteq G\) is non-emphy and for all \(a, b \in H\), \(a \cdot b^{-1} \in H\) then \(H \leq G\).
\end{lemma}

\begin{eg}\leavevmode
  \begin{enumerate}
  \item Additive groups: \((\N, +, 0)\), \((\R, +, 0)\), \((\C, +, 0)\).
  \item Groups of symmetries: \(S_n\), \(D_{2n}\), \(\GL_n(\R)\). They have subgroups \(A_n \leq S_n\), \(C_n \leq D_{2n}\), \(\SL_n(\R) \leq \GL_n(\R)\).
  \item An group \(G\) is \emph{abelian}\index{group!abelian} is a group such that \(a \cdot b = b \cdot a\) for all \(a, b \in G\).
  \end{enumerate}
\end{eg}

If \(H \leq G\), \(g \in G\), we define the \emph{left \(H\)-coset} of \(G\) to be
\[
  gH = \{gh: h \in H\}.
\]
As we have seen in IA Groups, the \(H\)-cosets form a patition of \(G\) and are in bijection with each other via
\begin{align*}
  H &\leftrightarrow gH \\
  h &\mapsto gh \\
  g^{-1}h &\mapsfrom h
\end{align*}
We write \(G/H\) for the set of left cosets.

\begin{theorem}[Lagrange]\index{Lagrange's Theorem}
  \label{thm:lagrange}
  If \(G\) is a finite group and \(H \leq G \) then
  \[
    |G| = |H| \cdot |G/H|.
  \]
\end{theorem}

We call \(|G/H|\) the \emph{index}\index{group!index} of \(H\) in \(G\).

\begin{definition}[Order]\index{order}
  Given \(g \in G\), the \emph{order} of \(g\) is the smallest \(n\) such that \(g^n = e\). We write \(n = o(g) = |g|\). If no such \(n\) exists then \(g\) has infinite order.
\end{definition}

Recall that if \(g^m = e\) then \(|g| \divides m\).

\begin{lemma}
  If \(G\) is finite and \(g \in G\) then \(|g| \divides |G|\).
\end{lemma}

\begin{proof}
  The set
  \[
    \generation g = \{e, g, \dots, g^{|g| - 1}\}
  \]
  is a subgroup of \(G\). The result follows from \nameref{thm:lagrange}.
\end{proof}

\subsection{Normal subgroups, Quotients and Homomorphisms}

Recall that \(gH = g'H\) if and only if \(g^{-1}g' \in H\). In particular, if \(h \in H\) then \(ghH = gH\).

Given a subgroup \(H \leq G\), we want to define a group structure on its cosets. Argurably the most natural candidate for the group operation would be
\begin{align*}
  - \cdot -: G/H \times G &\to G/H \\
  (gH, g'H) &\mapsto gg'H
\end{align*}
But is this well-defined? Suppose \(g'H = g'hH\), then
\[
  (gH) \cdot (g'hH) = gg'hH = gg'H
\]
so it is well-defined in the second coordinate. Suppose \(gH = ghH\), then
\[
  (ghH) \cdot (g'H) = ghg' H \stackrel{?}{=} gg'H
\]
where the last step holds if and only if \((g')^{-1}hg' \in H\) for all \(h \in H\), \(g' \in G\). Thus we need this true to define a group structure on the cosets. This motivates us to define

\begin{definition}[Normal subgroup]\index{group!subgroup!normal}
  A subgroup \(H \leq G\) is \emph{normal} if for all \(h \in H\), \(g \in G\), \(g^{-1}hg \in H\). Write \(H \normal G\).
\end{definition}

\begin{definition}[Quotient group]\index{group!quotient}
  If \(H \normal G\), then \(G/H\) equipped with the product
  \begin{align*}
    G/H \times G/H &\to G/H \\
    (gH, g'H) &\mapsto gg'H
  \end{align*}
  and identity \(eH\) is a group. This is the \emph{quotient group} of \(G\) by \(H\).
\end{definition}

Now we have defined and seen quite a few groups. We are interested not in the internal structure of groups but how they relate to each other. This motivates to define morphisms between groups:

\begin{definition}[Homomorphism]\index{group!homomorphism}
  If \((G, \cdot, e_G)\) and \((H, *, e_H)\) are groups, a function \(\varphi: G \to H\) is a \emph{homomorphism} if for all \(g, h \in G\),
  \[
    \varphi(g \cdot g') = \varphi(g) * \varphi(g').
  \]
\end{definition}

This implies that \(\varphi(e_G) = e_H\) and \(\varphi(g^{-1}) = \varphi(g)^{-1}\). We define
\begin{align*}
  \ker \varphi &= \{g \in G: \varphi(g) = e_H\}, \\
  \im \varphi &= \{\varphi(g): g \in G\}.
\end{align*}

\begin{lemma}\leavevmode
  \begin{itemize}
  \item \(\ker \varphi \normal G\),
  \item \(\im \varphi \leq H\).
  \end{itemize}
\end{lemma}

\begin{proof}
  Easy.
\end{proof}

\begin{definition}[Isomorphism]\index{group!isomorphism}
  A homomorphism \(\varphi\) is an \emph{isomorphism} if it is a bijection. Say \(G\) and \(H\) are \emph{isomorphic} if there exists some isomorphism \(\varphi: G \to H\). Write \(G \cong H\).
\end{definition}

\begin{ex}
  If \(\varphi\) is an isomorphism then the inverse \(\varphi^{-1}: H \to G\) is also an isomorphism.
\end{ex}

\begin{theorem}[First Isomorphism Theorem]\index{tbd}
  Let \(\varphi: G \to H\) be a homomorphism . Then \(\ker \varphi \leq G\), \(\im \varphi \leq G\) and
  \[
    G/\ker \varphi \cong \im \varphi.
  \]
\end{theorem}

\begin{proof}
  We have done the first part. For the second part, define
  \begin{align*}
    \theta: G/\ker \varphi &\to \im \varphi \\
    g\ker \varphi &\mapsto \varphi(g)
  \end{align*}
  \[
    \begin{tikzcd}
      G \ar[r, "\varphi"] \ar[d, two heads] & H \\
      G/\ker \varphi \ar[ur, dashed, "\phi"']
    \end{tikzcd}
  \]
  Check this is well-defined: if \(g\ker \varphi = g'\ker \varphi\) then \(g^{-1}g' \in \ker \varphi\) so \(e_H = \varphi(g^{-1}g') = \varphi(g)^{-1}\varphi(g')\), \(\varphi(g) = \varphi(g')\) and \(\theta(g\ker \varphi) = \theta(g'\ker \varphi)\).

  \(\theta\) is a homomorphism:
  \[
    \theta(g\ker \varphi \cdot g'\ker \varphi) = \theta(gg' \ker \varphi) = \varphi(gg') = \varphi(g)\varphi(g') = \theta(g\ker \varphi) \theta(g\ker \varphi).
  \]
  \(\theta\) is surjective and finally to show it is injective, suppose \(\theta(g\ker \varphi) = e_H\). Then \(g \in \ker \varphi\) so \(g\ker \varphi = e\ker \varphi\).
\end{proof}

\blindtext

\section{Rings}

\blindtext

\section{Modules}

\subsection{Definitions}

\begin{definition}[Module]\index{module}
  Let \(R\) be a commutative ring. A quadruple \((M, +, , 0_M, \cdot)\) is an \emph{\(R\)-module} if \((M, +, 0_M)\) is an abelian group and the operation \(- \cdot -: R \times M \to M\) satisfies
  \begin{itemize}
  \item \((r_1 + r_2) \cdot m = r_1 \cdot m + r_2 \cdot m\),
  \item \(r \cdot (m_1 + m_2) = r \cdot m_1 + r \cdot m_2\),
  \item \(r_2 \cdot (r_1 \cdot m) = (r_2r_2) \cdot m\),
  \item \(1_R \cdot m = m\).
  \end{itemize}
\end{definition}

\begin{eg}\leavevmode
  \begin{enumerate}
  \item If \(R = \F\) is a field then an \(\R\)-module is precisely an \(\F\)-vector space.
  \item For any ring \(R\), \(R^n = \underbrace{R \times \dots \times R}_{n \text{ times}}\) is an \(\R\)-module via
    \[
      r \cdot (r_1, \dots, r_n) = (rr_1, \dots, rr_n).
    \]
    In particular for \(n = 1\), \(R\) is an \(R\)-module.
  \item If \(I \ideal R\) then \(I\) is an \(R\)-module via
    \[
      r \cdot a = ra \in I.
    \]
    Also \(R/I\) is an \(\R\)-module via
    \[
      r \cdot (r_1 + I) = rr_1 + I \in R/I.
    \]
  \item For \(R = \Z\), an \(\R\)-module is precisely an abelian group. This is because the axiom for \(\cdot\) says that
    \begin{align*}
      - \cdot -: \Z \times M &\to M \\
      (n, m) &\mapsto
               \begin{cases}
                 \underbrace{m + \dots + m}_{n \text{ times}} & n \geq 0 \\
                 -(\underbrace{m + \dots + m}_{n \text{ times}}) & n < 0 \\
               \end{cases}
    \end{align*}
    so \(\cdot\) is uniquely determined by \(M\).
  \item Let \(\F\) be a field and \(V\) be a vector space over \(\F\). Let \(\alpha: V \to V\) be a linear map. Then we can make \(V\) into an \(\F[X]\)-module via
    \begin{align*}
      \F[X] \times V &\to V \\
      (f, v) &\mapsto f(\alpha)(v)
    \end{align*}
    Different \(\alpha\)'s make \(V\) into different \(\F[x]\)-modules.
  \item Restriction of scalars: if \(\varphi: R \to S\) is a ring homomorphism and \(M\) is an \(S\)-module, then \(M\) becomes an \(R\)-modules via
    \[
      r \cdot_R m = \varphi(r) \cdot_s m.
    \]
  \end{enumerate}
\end{eg}

\begin{definition}[Submodule]\index{module!submodule}
  If \(M\) is an \(\R\)-module, \(N \subseteq M\) is a \emph{submodule} if \(N\) is a subgroup of \((M, +, 0_M)\) and for any \(n \in N, r \in R\), \(r \cdot n \in N\). Write \(N \leq M\).
\end{definition}

\begin{eg}
  A subset of \(R\) is a submodule if and only if it is an ideal.
\end{eg}

\begin{definition}[Quotient module]\index{module!quotient}
  If \(N \leq M\) is a submodule, the \emph{quotient module} \(M/N\) is the set of \(N\)-cosets in \((M, +, 0_M)\), i.e. the quotient abelian group with
  \[
    r \cdot (m + N) = r \cdot m + N.
  \]
\end{definition}

\begin{definition}[Homomorphism]\index{module!homomorphism}
  A function \(f: M \to N\) is an \emph{\(\R\)-module homomorphism} if it is a homomorphism of abelian groups and \(f(r \cdot m) = r \cdot f(m)\).
\end{definition}

\begin{eg}
  If \(R = \F\) is a field and \(V\) and \(W\) are \(\F\)-modules (i.e. \(\F\)-vector spaces), then a map is an \(\F\)-module homomorphism if and only if it is an \(\F\)-linear map.
\end{eg}

\begin{theorem}[First Isomorphism Theorem]\index{tbd}
  If \(f: M \to N\) is an \(R\)-module homomorphism then
  \begin{align*}
    \ker f &= \{m \in M: f(m) = 0\} \leq M \\
    \im f &= \{n \in N: n = f(m)\} \leq N
  \end{align*}
  and
  \[
    M/\ker f \cong \im f.
  \]
\end{theorem}

\begin{theorem}[Second Isomorphism Theorem]\index{tbd}
  Let \(A, B \leq M\) be submodules. Then
  \begin{align*}
    A + B &= \{m \in M: m = a + b, a \in A, b \in B\} \leq M \\
    A \cap B &\leq M
  \end{align*}
  and
  \[
    (A + B)/A \cong B/(A \cap B).
  \]
\end{theorem}

\begin{theorem}[Third Isomorphism Theorem]\index{tbd}
  Let \(N \leq L \leq M\) be a chain of submodules. Then
  \[
    \frac{M/N}{L/N} \cong M/L.
  \]
\end{theorem}

\begin{definition}[Annihilator]\index{annihilator}
  If \(M\) is an \(R\)-module and \(m \in M\), the \emph{annihilator} of \(m\) is
  \[
    \Ann(m) = \{r \in R: r \cdot m = 0_M\} \ideal R.
  \]

  The \emph{annihilator} of \(M\) is
  \[
    \Ann(M) = \bigcap_{m \in M} \Ann(m) \ideal R.
  \]
\end{definition}

\begin{definition}[Generated submodule]\index{module!submodule!generated}
  If \(M\) is an \(R\)-module and \(m \in M\), the \emph{submodule generated by \(m\)} is
  \[
    Rm = \{r \cdot m \in M: r \in R\}.
  \]
\end{definition}

\begin{note}
  Intuitively, the annihilator of an element is the stabiliser of a ring action and that of a module is the kernel. We also have
  \[
    Rm \cong R/\Ann(m).
  \]
\end{note}

\begin{definition}[Finitely generated]\index{finitely generated}
  \(M\) is \emph{finitely generated} if there are \(m_1, \dots, m_n \in M\) such that
  \[
    M = Rm_1 + \dots Rm_n = \{r_1m_1 + \dots + r_nm_r: r_i \in R\}.
  \]
\end{definition}

\begin{lemma}
  An \(R\)-module \(M\) is finitely generated if and only if there is a surjetion \(\varphi: R^n \surj M\) for some \(n\).
\end{lemma}

\begin{proof}\leavevmode
  \begin{itemize}
  \item \(\Rightarrow\): Suppose \(M = Rm_1 + \dots + Rm_n\). Define
    \begin{align*}
      \varphi: R^n &\to M \\
      (r_1, \dots, r_n) &\mapsto r_1m_1 + \dots + r_nm_m
    \end{align*}
    This is an \(R\)-module homomorphism and is surjective.
  \item \(\Leftarrow\): Let \(m_i = \varphi((0, \dots, 0, 1, 0, \dots, 0))\) with \(1\) in the \(i\)th position. Then
    \begin{align*}
      \varphi((r_1, \dots, r_n)) &= \varphi((r_1, 0, \dots, 0) + \dots + (0, \dots, 0, r_n)) \\
                                 &= \varphi((r_1, 0, \dots, 0)) + \dots + \varphi((0, \dots, 0, r_n)) \\
                                 &= r_1 \varphi((1, 0, \dots, 0)) + \dots + r_n \varphi((0, \dots, 0, 1)) \\
      &= r_1m_1 + \dots + r_nm_n
    \end{align*}
    As \(\varphi\) is surjective, \(M = Rm_1 + Rm_n\).
  \end{itemize}
\end{proof}

\begin{corollary}
  Let \(M\) be an \(R\)-module and \(N \leq M\). If \(M\) is finitely generated the so is \(M/N\).
\end{corollary}

\begin{proof}
  \[
    R^n \overset{f}{\surj} M \overset{\pi}{\surj} M/N.
  \]
\end{proof}

\begin{note}
  A module of a finitely generated \(R\)-module need \emph{not} to be finitely generated. For example,
  \[
    (X_1, X_2, \dots) \ideal \Z[X_1, X_2, \dots] = R
  \]
  is an \(R\)-module but note finitely generated, as otherwise it would be a finitely generated ideal.
\end{note}

\begin{eg}
  For \(\alpha \in \C\), \(\alpha\) is an algebraic integer if and only if \(\Z[\alpha]\) is a finitely generated \(\Z\)-module.
\end{eg}

\subsection{Direct Sums and Free Modules}

\begin{definition}[Direct sum]\index{direct sum}
  If \(M_1, \dots, M_k\) are \(R\)-modules, the \emph{direct sum} \(M_1 \oplus \dots \oplus M_k\) is the set \(M_1 \times \dots \times M_k\) with addition
  \[
    (m_1, \dots, m_k) + (m_1', \dots, m_k') = (m_1 + m_1', \dots, m_k + m_k')
  \]
  and \(R\)-module structure
  \[
    r \cdot (m_1, \dots, m_k) = (rm_1, \dots, rm_k).
  \]
\end{definition}

\begin{eg}
  \[
    R^n = \underbrace{R \oplus \dots \oplus R}_{n \text{ times}}.
  \]
\end{eg}

\begin{definition}[Independence]\index{independenc}
  Let \(m_1, \dots m_k \in M\). They are \emph{independent} if
  \[
    \sum_i r_i \cdot m_i = 0
  \]
  implies that \(r_i = 0\) for all \(1 \leq i \leq k\).
\end{definition}

\begin{definition}[Free generation]\index{tbd}
  A subset \(S \subseteq M\) \emph{generates \(M\) freely} if
    \begin{enumerate}
    \item \(S\) generates \(M\).
    \item Any function \(\psi: S \to N\) to an \(R\)-module \(N\) extends to an \(R\)-module homomorphism \(\theta: M \to N\).
    \end{enumerate}
    \[
      \begin{tikzcd}
        S \ar[r, hook] \ar[dr, "\psi"'] & R^S \ar[d, dashed, "\theta"] \\
        & N
      \end{tikzcd}
    \]
\end{definition}

\begin{note}
  We can show this extension is unique: given \(\theta_1, \theta_2: M \to N\) two extensions of \(\psi\), \(\theta_1 - \theta_2:M \to N\) is an \(R\)-module homomorphism so \(\ker(\theta_1 - \theta_2) \leq M\). But \(\theta_1, \theta_2\) both extend \(\psi\) so \(S \subseteq \ker(\theta_1 - \theta_2)\). As \(S\) generates \(M\), \(M \leq \ker(\theta_1 - \theta_2)\) so \(\theta_1 = \theta_2\).
\end{note}

An \(R\)-module which is freely generated by \(S \subseteq M\) is said to be \emph{free} and \(S\) is called a \emph{basis}

\begin{proposition}
  For a finite subset \(S = \{m_1, \dots, m_k\} \subseteq M\), TFAE:
  \begin{enumerate}
  \item \(M\) is freely generated by \(S\).
  \item \(M\) is generated by \(S\) and \(S\) is independent.
  \item Every \(m \in M\) can be written as \(r_1m_1 + \dots + r_km_k\) for some unique \(r_i \in R\).
  \end{enumerate}
\end{proposition}

\begin{proof}\leavevmode
  \begin{itemize}
  \item \(1 \Rightarrow 2\): Let \(S\) generate \(M\) freely. If \(S\) is not independent, then there is a non-trivial relation
    \[
      \sum_{i = 1}^k r_im_i = 0
    \]
    with \(r_j \neq 0\). Let
    \begin{align*}
      \psi: S &\to R \\
      m_i &\mapsto
            \begin{cases}
              0_R & i \neq j \\
              1_R & i = j
            \end{cases}
    \end{align*}
    This extends to an \(R\)-module homomorphism \(\theta: M \to R\). Then
    \[
      0 = \theta(0) = \theta \left(\sum r_im_i \right) = \sum r_i\theta(m_i) = r_j.
    \]
    Absurd. Thus \(S\) is independent.
  \item The other steps follow similarly from those in IB Linear Algebra.
  \end{itemize}
\end{proof}

\begin{eg}
  Unlike vector spaces, a minimal generating set need not to be independent. For example \(\{2, 3\} \subseteq \Z\) generates \(\Z\) but is not linear independent as \((-3) \cdot 2 + (2) \cdot 3 = 0\).
\end{eg}

However, like vector spaces, in case a module is freely generated, it is isomorphic to direct sums of copies of the ring:

\begin{lemma}
  If \(S = \{m_1, \dots, m_k\} \subseteq M\) freely generates \(M\) then
  \[
    M \cong R^k
  \]
  as an \(R\)-module.
\end{lemma}

\begin{proof}
  This is entirely analogous to vector spaces. Let
  \begin{align*}
    f: R^k &\to M \\
    (r_1, \dots, r_k) &\mapsto \sum_i r_im_i
  \end{align*}
  It is surjective as \(S\) generates \(M\) and injective as \(m_i\)'s are independent.
\end{proof}

If an \(R\)-module is generated by \(m_1, \dots, m_k\), we have seen before that there is a surjection \(f: R^k \surj M\). We define

\begin{definition}[Relation module]\index{relation module}
  The \emph{relation module} for the generators is
  \[
    \ker f \leq \R^k.
  \]
\end{definition}

As \(M \cong R^k/\ker f\), knowing \(M\) is equivalent to knowing the relation module.

\begin{definition}[Finitely presented]\index{finitely presented}
  \(M\) is \emph{finitely presented} if there is a finitely generating set \(m_1, \dots, m_k\) for which the associated relation module is finitely generated.
\end{definition}

Let \(\{n_1, \dots, n_r\} \subseteq \ker f \leq R^k\) be a set of generators. Then
\[
  n_i =
  \begin{pmatrix}
    r_{1i} \\
    r_{ri} \\
    \vdots \\
    r_{ki}
  \end{pmatrix}
\]
and \(M\) is generated by \(m_1, \dots, m_k\) subject to relations
\[
  \sum_{j = 1}^k r_{ij} m_j = 0
\]
for \(1 \leq i\leq r\).

\begin{proposition}[Invariance of Dimension]
  If \(R^n \cong R^m\) then \(n = m\).
\end{proposition}

\begin{note}
  This does not hold in general for modules over non-commutative rings.
\end{note}

\begin{proof}
  As a general strategy, let \(I \ideal R\). Then
  \[
    IM = \left\{\sum a_im_i: a_i \in I, m_i \in M \right\} \leq M
  \]
  is a submodule as
  \[
    r \cdot \sum a_im_i = \sum (ra_i)m_i \in IM.
  \]
  Thus we have a quotient \(R\)-module \(M/IM\). We can make this into an \((R/I)\)-module via
  \[
    (r + I) \cdot (m + IM) = rm + IM.
  \]

  Let \(I \ideal R\) be a maximal proper ideal (this requires Zorn's Lemma). Then \(R/I\) is a field and therefore \(R^n \cong R^m\) implies
  \begin{align*}
    R^n/IR^n &\cong R^m/IR^m \\
    (R/I)^n &\cong (R/I)^m
  \end{align*}
  This is a vector space isomorphism so \(n = m\).
\end{proof}

We have classified all finite abelian groups (well, at least we declared so), i.e.\ \(\Z\)-modules. What if we want to classify all \(R\)-modules? That is going to be the final goal we will build towards.

Recall that \(M\) is finitely generated by \(m_1, \dots, m_k\) if and only if there is a surjection \(f: R^k \surj M\). \(M\) is finitely presentely if and only \(\ker f\) is finitely generated, say \(n_1, \dots, n_\ell\). Let
\[
  n_i =
  \begin{pmatrix}
    r_{1i} \\
    r_{ri} \\
    \vdots \\
    r_{ki}
  \end{pmatrix}
\]
then such an \(R\)-module \(M\) is determined by the matrix
\[
  \begin{pmatrix}
    r_{11} & r_{12} & \cdots & r_{1\ell} \\
    r_{r1} & & & \\
    \vdots & & \ddots & \\
    r_{k1} & & & r_{k\ell}
  \end{pmatrix}
  \in \matrixring_{k, \ell}(R).
\]

\subsection{Matrices over Euclidean Domains}

For this section assume \(R\) to be a Euclidean domain and let \(\varphi: R \setminus \{0\} \to \Z_{\geq 0}\) be the Euclidean function. For \(a, b \in R\), we have shown that \(\gcd(a, b)\) exists and is unique up to associates. In addition, the Euclidean algorithm shows that \(\gcd(a, b) = ax + by\) for some \(x, y \in R\).

What follows would be very similar to what we have learned in IB Linear Algebra --- in fact identical except at one place:

\begin{definition}[Elementary row operation]\index{tbd}
  \emph{Elementary row operation} on an \(m \times n\) matrix \(m\) with entries in \(R\) are
\end{definition}
\printindex
\end{document}
